data/isabelle/src/ESPLogic/WeakTyping.thy
@@ -43,7 +43,7 @@ definition approx :: "typing \<Rightarrow> state set"
 where "approx typing \<equiv> {q. case q of (t,r,s) \<Rightarrow>
   \<forall> (i,step) \<in> steps t. 
     \<forall> R. roleMap r i = Some R \<longrightarrow>
-      (\<forall> n. MVar n \<in> FV_rolestep step \<longrightarrow>
+      (\<forall> n. MVar n \<in> FV_rolestep step \<and> n \<notin> wildcards R step \<longrightarrow>
          s (MVar n, i) \<in> typing (R, n) i (t,r,s)
       )}"
 
@@ -63,7 +63,7 @@ lemma approx_unfold:
   "((t,r,s) \<in> approx typing) = 
    (\<forall> (i,step) \<in> steps t. 
       \<forall> R. roleMap r i = Some R \<longrightarrow>
-        (\<forall> n. MVar n \<in> FV_rolestep step \<longrightarrow>
+        (\<forall> n. MVar n \<in> FV_rolestep step \<and> n \<notin> wildcards R step \<longrightarrow>
            s (MVar n, i) \<in> typing (R, n) i (t,r,s)))"
 by (auto simp: approx_def)
 
@@ -72,7 +72,8 @@ lemma in_approxI:
     "\<And> i step R n.
      \<lbrakk> (i,step) \<in> steps t;
        roleMap r i = Some R;
-       MVar n \<in> FV_rolestep step
+       MVar n \<in> FV_rolestep step;
+       n \<notin> wildcards R step
      \<rbrakk>
        \<Longrightarrow> s (MV n i) \<in> typing (R, n) i (t,r,s)"
   shows "(t,r,s) \<in> approx typing"
@@ -83,6 +84,7 @@ lemma in_approxD:
   and asms: "(i,step) \<in> steps t"
             "roleMap r i = Some R"
             "MVar n \<in> FV_rolestep step"
+            "n \<notin> wildcards R step"
   shows "s (MV n i) \<in> typing (R, n) i (t,r,s)"
 using approx asms
 by (auto simp: approx_unfold)
@@ -251,10 +253,12 @@ lemma (in reachable_thread) step_done_typing:
   assumes typ_rule:
     "\<And> step.
      \<lbrakk> (i, step) \<in> steps t;
-       MVar v \<in> FV_rolestep step
+       MVar v \<in> FV_rolestep step;
+       v \<notin> wildcards (done @ todo) step
      \<rbrakk> \<Longrightarrow> s (MV v i) \<in> typing (done @ todo, v) i (t, r, s)"
   and step_done: "step \<in> set done"
   and step_var: "MVar v \<in> FV_rolestep step"
+                "v \<notin> wildcards (done @ todo) step"
   shows "s (MV v i) \<in> typing (done @ todo, v) i (t, r, s)"
 proof (cases "step \<in> skipped")
   case False
@@ -276,7 +280,7 @@ next
     where roleBefore: "listOrd (done@todo) step' (Note l ty pt)"
     and varSourced: "v \<in> sourced_vars step'"
     by auto
-  hence varOfRecv: "MVar v \<in> FV_rolestep step'" by auto
+  hence notWildcard: "v \<notin> wildcards (done @ todo) step'" by auto
   have notNote: "\<not> noteStep step'" using varSourced by auto
   have "step' \<in> set done" 
     using roleBefore step_done noteEq
@@ -290,10 +294,10 @@ next
     by(auto dest: done_notin_todoD)
   hence "(i, step') \<in> steps t" using notNote by (cases step', auto)
   thus ?thesis
-    using varOfRecv by (auto intro!: typ_rule thread_exists)
+    using varSourced notWildcard by (auto intro!: typ_rule thread_exists)
 qed
 
-(* TODO ? *)
+
 definition typing_A_ext :: "typing \<Rightarrow> (role \<times> varid) \<Rightarrow> msgtype"
 where "typing_A_ext typing rv \<equiv> case rv of
     (r, MVar n) \<Rightarrow> typing (r, n)
@@ -314,7 +318,8 @@ proof -
     hence "n \<in> used_vars step" using match by auto
     then obtain sstep where "n \<in> sourced_vars sstep" and sstep: "(i, sstep) \<in> steps t"
       using todo_step thread_exists by (auto dest: source_step)
-    hence sources: "MVar n \<in> FV_rolestep sstep" by auto
+    hence sources: "MVar n \<in> FV_rolestep sstep"
+                   "n \<notin> wildcards (done@todo) sstep" by auto
     have "s (MVar n, i) \<in> typing (done@todo, n) i (t,r,s)"
       using sstep thread_exists sources approx
       apply -
@@ -335,7 +340,7 @@ lemma (in reachable_state) reachable_in_approxI:
        (done, step # todo) \<in> set (splits R);
        \<not> sendStep step; \<not> noteStep step;
        n \<in> sourced_vars step;
-       \<forall> step' \<in> set done. MVar n \<notin> FV_rolestep step';
+       \<forall> step' \<in> set done. MVar n \<in> FV_rolestep step' \<longrightarrow> n \<in> wildcards R step';
        hint ''completenessCase'' (step, n);
        
        (t,r,s) \<in> reachable P;
@@ -353,7 +358,8 @@ proof -
     have
      "\<lbrakk> r i = Some (done, todo, skipped);
         (i,step) \<in> steps t;
-        MVar n \<in> FV_rolestep step
+        MVar n \<in> FV_rolestep step;
+        n \<notin> wildcards (done@todo) step
       \<rbrakk> \<Longrightarrow> s (MV n i) \<in> typing (done@todo, n) i (t,r,s)"
     proof(induct arbitrary: i "done" todo step n skipped rule: reachable_induct)
       case (send t r s i "done" l pt todo skipped m i' done' todo' step n skipped')
@@ -415,11 +421,13 @@ proof -
         hence cur_thread: "?role = done' @ todo'" "i = i'" 
           using recv by auto
         have ?case
-        proof(cases "\<exists> step' \<in> set done.  MVar n \<in> FV_rolestep step'")
+        proof(cases "\<exists> step' \<in> set done.
+                       MVar n \<in> FV_rolestep step' \<and> n \<notin> wildcards (done'@todo') step'")
           case True
           with recv
           obtain step'
             where FV: "MVar n \<in> FV_rolestep step'" 
+            and notWildcard: "n \<notin> wildcards (done'@todo') step'"
             and step': "step' \<in> set done"
             by auto
           hence "s (MV n i) \<in> typing (done'@todo', n) i (t, r, s)"
@@ -541,11 +549,13 @@ proof -
           next
             assume "n \<in> sourced_vars step"
             thus ?thesis
-            proof (cases "\<exists> step' \<in> set done.  MVar n \<in> FV_rolestep step'")
+            proof (cases "\<exists> step' \<in> set done.
+                            MVar n \<in> FV_rolestep step' \<and> n \<notin> wildcards (done'@todo') step'")
               case True
               with match
               obtain step'
                 where FV: "MVar n \<in> FV_rolestep step'"
+                and notWildcard: "n \<notin> wildcards (done'@todo') step'"
                 and step': "step' \<in> set done"
                 by auto
               hence "s (MV n i) \<in> typing (done'@todo', n) i (t, r, s)"
@@ -580,13 +590,35 @@ proof -
           qed
 
         next
-          case False
-          moreover note `?new`
-          moreover hence "n \<in> used_vars step" using match False by auto
-          ultimately obtain step' 
+          case False note notMatch = this
+          have role_split: "done'@todo' = ?role" "done' = done @ [step]"
+            using match `?new` by auto
+          have "\<exists> st. (i, st) \<in> steps t \<and> n \<in> sourced_vars st" proof (cases "n \<in> FMV pt")
+            case True
+            with match notMatch `?new` obtain step'
+              where source_ord: "listOrd (done'@todo') step' step"
+                and sourced: "n \<in> sourced_vars step'"
+              by auto
+            have "step' \<in> set done" proof -
+              have "wf_role ?role" using match by (auto intro: th1.role_in_P wf_roles)
+              hence "distinct ?role" unfolding wf_role_def distinct_list_def by simp
+              thus ?thesis using role_split source_ord
+                by (auto intro: in_set_listOrd1 in_set_listOrd2)
+            qed
+            hence "(i, step') \<in> steps t" using sourced
+              by (auto dest!: th1.in_steps_eq_in_done th1.note_in_skipped)
+            thus ?thesis using sourced by blast
+          next
+            case False
+            hence "MVar n = mv" using match `?new` by auto
+            hence "n \<in> used_vars step" using notMatch `?new` by auto
+            thus ?thesis using match `?new`
+              by (fastforce dest!: th1.source_step[OF th1.thread_exists])
+          qed
+          then obtain step'
             where "(i, step') \<in> steps t" 
                   "n \<in> sourced_vars step'"   
-            by (fastforce dest!: th1.source_step[OF th1.thread_exists])
+            by auto
           hence typed: "s (MV n i) \<in> typing (?role, n) i (t, r, s)"
             by (auto dest: IH[OF th1.thread_exists])
           have "done'@todo' = ?role" using match `?new` by auto
@@ -635,9 +667,13 @@ proof(induct rule: reachable_in_approxI[OF monoTyp])
   case (1 t r s i "done" todo skipped m R step n)
   { fix v V
     assume "v \<in> V"
-      and "\<forall>step'\<in>set done. MVar v \<notin> FV_rolestep step'"
+      and "\<forall>step'\<in>set done. MVar v \<in> FV_rolestep step' \<longrightarrow> v \<in> wildcards R step'"
     hence "v \<in> foldl (\<lambda> fv step'. fv - sourced_vars step') V done"
-      by (induct "done" arbitrary: V, auto intro!: sourced_imp_FV)
+      proof (induct "done" arbitrary: V)
+        case (Cons st)
+        hence "v \<notin> sourced_vars st" by (auto intro!: sourced_imp_FV)
+        thus ?case using Cons by simp
+      qed simp
   }
   hence "n \<in> foldl (\<lambda> fv step'. fv - sourced_vars step') (sourced_vars step) done"
   using 1 by auto
